Tests/AllTests.lean
@@ -81,6 +81,7 @@ import Tests.Compiler.ShippingScalarSoundnessTest
 import Tests.Compiler.FreshNameSoundnessTest
 import Tests.Compiler.ShippingBindingsSoundnessTest
 import Tests.Compiler.ShippingCacheSoundnessTest
+import Tests.Compiler.ShippingTranslateSoundnessTest
 import Tests.CircuitDoTest
 import Tests.RunCircuitHTest
 import Tests.TestCppSim
